examples/layeredeffects/Alg.fst
@@ -766,6 +766,9 @@ let rec fixup_no_other (l:op{Other? l}) (ls:list baseop)
     | [] -> ()
     | l1::ls -> fixup_no_other l ls
 
+let lattice_put (s:state) () : L.EFF unit [L.WR] =
+  L.put s
+
 // This would be a lot nicer if it was done in L.EFF itself,
 // but the termination proof fails since it has no logical payload.
 let rec interp_into_lattice_tree #a (#labs:list baseop)
@@ -774,10 +777,10 @@ let rec interp_into_lattice_tree #a (#labs:list baseop)
   = match t with
     | Return x -> L.return _ x
     | Op Read i k ->
-      L.bind _ _ _ _ (reify (L.get i))
+      L.bind _ _ _ _ (reify (L.get ()))
        (fun x -> interp_into_lattice_tree #a #labs (k x))
     | Op Write i k ->
-      L.bind _ _ _ _ (reify (L.put i))
+      L.bind _ _ _ _ (reify (lattice_put i ()))
        (fun x -> interp_into_lattice_tree #a #labs (k x))
     | Op Raise i k ->
       L.bind _ _ _ _ (reify (L.raise ()))
@@ -785,6 +788,7 @@ let rec interp_into_lattice_tree #a (#labs:list baseop)
 
 let interp_into_lattice #a (#labs:list baseop)
   (f : unit -> Alg a (fixup labs))
+  ()
   : Lattice.EFF a (trlabs labs)
   = Lattice.EFF?.reflect (interp_into_lattice_tree (reify (f ())))
 
@@ -793,7 +797,7 @@ let interp_into_lattice #a (#labs:list baseop)
 let interp_full #a (#labs:list baseop)
   (f : unit -> Alg a (fixup labs))
   : Tot (f:(state -> Tot (option a & state)){Lattice.abides f (Lattice.interp (trlabs labs))})
-  = reify (interp_into_lattice #a #labs f)
+  = reify (interp_into_lattice #a #labs f ())
 
 
 (* Doing it directly. *)
